src/promotion/iPromotionDef.v
@@ -1,0 +1,186 @@
+Require Import Omega.
+Require Import RelationClasses.
+
+From sflib Require Import sflib.
+From Paco Require Import paco.
+
+From PromisingLib Require Import Axioms.
+From PromisingLib Require Import Basic.
+From PromisingLib Require Import DataStructure.
+From PromisingLib Require Import DenseOrder.
+From PromisingLib Require Import Loc.
+From PromisingLib Require Import Language.
+
+Require Import Event.
+Require Import Time.
+Require Import View.
+Require Import Cell.
+Require Import Memory.
+Require Import TView.
+Require Import Local.
+Require Import Thread.
+Require Import Configuration.
+
+Require Import ITreeLang.
+
+Require Import PromiseConsistent.
+
+Set Implicit Arguments.
+
+
+(* promotion *)
+
+(* we can use interp_state, but we define it directly to avoid unnecessary taus *)
+CoFixpoint promote_itree (l: Loc.t) (st: Const.t) R (itr: itree MemE.t R): itree MemE.t (Const.t * R) :=
+  match (observe itr) with
+  | RetF r => Ret (st, r)
+  | TauF itr' => tau;;(promote_itree l st itr')
+  | VisF (MemE.read loc ord) k =>
+    if Loc.eq_dec loc l
+    then tau;;(promote_itree l st (k st))
+    else Vis (MemE.read loc ord) (fun r => promote_itree l st (k r))
+  | VisF (MemE.write loc val ord) k =>
+    if Loc.eq_dec loc l
+    then tau;;(promote_itree l val (k tt))
+    else Vis (MemE.write loc val ord) (fun r => promote_itree l st (k r))
+  | VisF (MemE.update loc (MemE.fetch_add addendum) ordr ordw) k =>
+    if Loc.eq_dec loc l
+    then tau;;(promote_itree l (st + addendum) (k (st + addendum)))
+    else Vis (MemE.update loc (MemE.fetch_add addendum) ordr ordw) (fun r => promote_itree l st (k r))
+  | VisF (MemE.update loc (MemE.cas old new) ordr ordw) k =>
+    if Loc.eq_dec loc l
+    then tau;; (if (Const.eq_dec st old)
+                then promote_itree l 1 (k new)
+                else promote_itree l 0 (k st))
+    else Vis (MemE.update loc (MemE.cas old new) ordr ordw) (fun r => promote_itree l st (k r))
+  | VisF e k => Vis e (fun r => promote_itree l st (k r))
+  end.
+
+Lemma unfold_promote_itree l st R (itr: itree MemE.t R):
+  promote_itree l st itr =
+  match (observe itr) with
+  | RetF r => Ret (st, r)
+  | TauF itr' => tau;;(promote_itree l st itr')
+  | VisF (MemE.read loc ord) k =>
+    if Loc.eq_dec loc l
+    then tau;;(promote_itree l st (k st))
+    else Vis (MemE.read loc ord) (fun r => promote_itree l st (k r))
+  | VisF (MemE.write loc val ord) k =>
+    if Loc.eq_dec loc l
+    then tau;;(promote_itree l val (k tt))
+    else Vis (MemE.write loc val ord) (fun r => promote_itree l st (k r))
+  | VisF (MemE.update loc (MemE.fetch_add addendum) ordr ordw) k =>
+    if Loc.eq_dec loc l
+    then tau;;(promote_itree l (st + addendum) (k (st + addendum)))
+    else Vis (MemE.update loc (MemE.fetch_add addendum) ordr ordw) (fun r => promote_itree l st (k r))
+  | VisF (MemE.update loc (MemE.cas old new) ordr ordw) k =>
+    if Loc.eq_dec loc l
+    then tau;; (if (Const.eq_dec st old)
+                then promote_itree l 1 (k new)
+                else promote_itree l 0 (k st))
+    else Vis (MemE.update loc (MemE.cas old new) ordr ordw) (fun r => promote_itree l st (k r))
+  | VisF e k => Vis e (fun r => promote_itree l st (k r))
+  end.
+Proof.
+  apply bisim_is_eq. ginit. gstep. red. refl.
+Qed.
+
+
+(* loc_free *)
+
+Definition loc_free_event (l: Loc.t) R (i: MemE.t R): Prop :=
+  match i with
+  | MemE.read loc _
+  | MemE.write loc _ _
+  | MemE.update loc _ _ _ => loc <> l
+  | _ => True
+  end.
+
+Variant _loc_free_itree l (loc_free_itree: forall R, itree MemE.t R -> Prop):
+  forall R, itree MemE.t R -> Prop :=
+| loc_free_itree_ret
+    R (r: R)
+  :
+    _loc_free_itree l loc_free_itree (Ret r)
+| loc_free_itree_tau
+    R (itr: itree MemE.t R) (LOCFREE: loc_free_itree R itr)
+  :
+    _loc_free_itree l loc_free_itree (tau;;itr)
+| loc_free_itree_vis
+    R X (e: MemE.t X) k
+    (LOCFREE1: loc_free_event l e)
+    (LOCFREE2: forall x, loc_free_itree R (k x))
+  :
+    _loc_free_itree l loc_free_itree (Vis e k)
+.
+#[export] Hint Constructors _loc_free_itree: core.
+
+Lemma loc_free_itree_mon l: monotone2 (_loc_free_itree l).
+Proof.
+  ii. destruct IN; eauto.
+Qed.
+#[export] Hint Resolve loc_free_itree_mon: paco.
+
+Definition loc_free_itree l := paco2 (_loc_free_itree l) bot2.
+
+Lemma promote_itree_loc_free l st R (itr: itree MemE.t R):
+  loc_free_itree l (promote_itree l st itr).
+Proof.
+  revert st itr. pcofix CIH. i. pfold. ides itr.
+  { rewrite unfold_promote_itree. econs. }
+  { rewrite unfold_promote_itree. econs. right. auto. }
+  { rewrite unfold_promote_itree. destruct e; ss.
+    { des_ifs.
+      { econs. right. auto. }
+      { econs; auto. }
+    }
+    { des_ifs.
+      { econs. right. auto. }
+      { econs; auto. }
+    }
+    { des_ifs.
+      { econs. right. auto. }
+      { econs; auto. }
+      { econs. right. auto. }
+      { econs; auto. }
+      { econs; auto. }
+    }
+    { econs; auto. ss. }
+    { econs; auto. ss. }
+    { econs; auto. ss. }
+    { econs; auto. ss. }
+  }
+Qed.
+
+Lemma step_loc_free
+      l e R (itr1 itr2: itree MemE.t R)
+      (LOCFREE: loc_free_itree l itr1)
+      (STEP: ILang.step e itr1 itr2):
+  loc_free_itree l itr2.
+Proof.
+  punfold LOCFREE.
+  destruct STEP; subst; dependent destruction LOCFREE; pclearbot; auto.
+  - apply LOCFREE2.
+  - apply LOCFREE2.
+  - apply LOCFREE2.
+  - apply LOCFREE2.
+  - apply LOCFREE2.
+  - apply LOCFREE2.
+  - apply LOCFREE2.
+  - pcofix CIH. pfold. rewrite unfold_spin. econs. auto.
+Qed.
+
+Lemma loc_free_step_is_accessing_loc
+      l e R (itr1 itr2: itree MemE.t R)
+      (LOCFREE: loc_free_itree l itr1)
+      (STEP: ILang.step (ThreadEvent.get_program_event e) itr1 itr2):
+  ~ ThreadEvent.is_accessing_loc l e.
+Proof.
+  punfold LOCFREE.
+  inv STEP; try (by destruct e); ss;
+    dependent destruction LOCFREE.
+  - destruct e; ss. clarify.
+  - destruct e; ss. clarify.
+  - destruct e; ss. clarify.
+  - destruct e; ss. clarify.
+Qed.
